src/Std/Data/DHashMap/Internal/RawLemmas.lean
@@ -70,9 +70,10 @@ variable [BEq α] [Hashable α]
 /-- Internal implementation detail of the hash map -/
 scoped macro "wf_trivial" : tactic => `(tactic|
   repeat (first
-    | apply Raw₀.wfImp_insert | apply Raw₀.wfImp_insertIfNew | apply Raw₀.wfImp_insertMany | apply Raw₀.Const.wfImp_insertMany| apply Raw₀.Const.wfImp_insertManyIfNewUnit | apply Raw₀.wfImp_erase
-    | apply Raw.WF.out | assumption | apply Raw₀.wfImp_empty | apply Raw.WFImp.distinct
-    | apply Raw.WF.empty₀))
+    | apply Raw₀.wfImp_insert | apply Raw₀.wfImp_insertIfNew | apply Raw₀.wfImp_insertMany
+    | apply Raw₀.Const.wfImp_insertMany| apply Raw₀.Const.wfImp_insertManyIfNewUnit
+    | apply Raw₀.wfImp_erase | apply Raw.WF.out | assumption | apply Raw₀.wfImp_empty
+    | apply Raw.WFImp.distinct | apply Raw.WF.empty₀))
 
 /-- Internal implementation detail of the hash map -/
 scoped macro "empty" : tactic => `(tactic| { intros; simp_all [List.isEmpty_iff] } )
@@ -90,8 +91,9 @@ private def queryNames : Array Name :=
     ``Raw.pairwise_keys_iff_pairwise_keys]
 
 private def modifyNames : Array Name :=
-  #[``toListModel_insert, ``toListModel_erase, ``toListModel_insertIfNew, ``toListModel_insertMany_list,
-  ``Const.toListModel_insertMany_list, ``Const.toListModel_insertManyIfNewUnit_list]
+  #[``toListModel_insert, ``toListModel_erase, ``toListModel_insertIfNew,
+  ``toListModel_insertMany_list, ``Const.toListModel_insertMany_list,
+  ``Const.toListModel_insertManyIfNewUnit_list]
 
 private def congrNames : MacroM (Array (TSyntax `term)) := do
   return #[← `(_root_.List.Perm.isEmpty_eq), ← `(containsKey_of_perm),
@@ -841,381 +843,370 @@ theorem distinct_keys [EquivBEq α] [LawfulHashable α] (h : m.1.WF) :
   simp_to_model using (Raw.WF.out h).distinct.distinct
 
 @[simp]
-theorem insertMany_list_nil :
+theorem insertMany_nil :
     m.insertMany [] = m := by
   simp [insertMany, Id.run]
 
 @[simp]
-theorem insertMany_list_singleton [EquivBEq α] [LawfulHashable α] {k : α} {v : β k} :
-    m.insertMany [⟨k,v⟩] = m.insert k v := by
+theorem insertMany_list_singleton {k : α} {v : β k} :
+    m.insertMany [⟨k, v⟩] = m.insert k v := by
   simp [insertMany, Id.run]
 
-theorem insertMany_list_cons {l : List ((a : α) × (β a))} {k : α} {v : β k} :
-    (m.insertMany (⟨k,v⟩ :: l)).1 = ((m.insert k v).insertMany l).1 := by
+theorem insertMany_cons {l : List ((a : α) × β a)} {k : α} {v : β k} :
+    (m.insertMany (⟨k, v⟩ :: l)).1 = ((m.insert k v).insertMany l).1 := by
   simp only [insertMany_eq_insertListₘ]
   cases l with
   | nil => simp [insertListₘ]
   | cons hd tl => simp [insertListₘ]
 
-theorem contains_insertMany_list [EquivBEq α] [LawfulHashable α] (h : m.1.WF) {l : List ((a : α) × (β a))} {k : α} :
+theorem contains_insertMany_list [EquivBEq α] [LawfulHashable α] (h : m.1.WF)
+    {l : List ((a : α) × β a)} {k : α} :
     (m.insertMany l).1.contains k = (m.contains k || (l.map Sigma.fst).contains k) := by
   simp_to_model using List.containsKey_insertList
 
-theorem contains_of_contains_insertMany_list [EquivBEq α] [LawfulHashable α] (h : m.1.WF) {l : List ((a : α) × (β a))} {k : α} :
+theorem contains_of_contains_insertMany_list [EquivBEq α] [LawfulHashable α] (h : m.1.WF)
+    {l : List ((a : α) × β a)} {k : α} :
     (m.insertMany l).1.contains k → (l.map Sigma.fst).contains k = false → m.contains k := by
   simp_to_model using List.containsKey_of_containsKey_insertList
 
-theorem get?_insertMany_list_not_mem [LawfulBEq α]
-    {l : List ((a : α) × (β a))} {k : α}
-    {not_mem : (l.map (Sigma.fst)).contains k = false}
-    (h : m.1.WF) :
+theorem get?_insertMany_list_of_contains_eq_false [LawfulBEq α] (h : m.1.WF)
+    {l : List ((a : α) × β a)} {k : α}
+    (h' : (l.map (Sigma.fst)).contains k = false) :
     (m.insertMany l).1.get? k = m.get? k := by
-  simp_to_model using getValueCast?_insertList_not_mem
+  simp_to_model using getValueCast?_insertList_of_contains_eq_false
 
-theorem get?_insertMany_list_mem [LawfulBEq α]
-    {l : List ((a : α) × (β a))} {k k' : α} {k_eq : k == k'} {v : β k}
-    {distinct : l.Pairwise (fun a b => (a.1 == b.1) = false)}
-    {mem : ⟨k,v⟩ ∈ l}
-    (h : m.1.WF) :
-    (m.insertMany l).1.get? k' = some (cast (by congr; apply LawfulBEq.eq_of_beq k_eq) v) := by
-  simp_to_model using getValueCast?_insertList_mem
+theorem get?_insertMany_list_of_mem [LawfulBEq α] (h : m.1.WF)
+    {l : List ((a : α) × β a)} {k k' : α} (k_beq : k == k') {v : β k}
+    (distinct : l.Pairwise (fun a b => (a.1 == b.1) = false))
+    (mem : ⟨k, v⟩ ∈ l) :
+    (m.insertMany l).1.get? k' = some (cast (by congr; apply LawfulBEq.eq_of_beq k_beq) v) := by
+  simp_to_model using getValueCast?_insertList_of_mem
 
-theorem get_insertMany_list_not_mem [LawfulBEq α]
-    {l : List ((a : α) × (β a))} {k : α}
-    {not_mem : (l.map (Sigma.fst)).contains k = false}
-    {h'}
-    (h : m.1.WF) :
-    (m.insertMany l).1.get k h' = m.get k (contains_of_contains_insertMany_list _ h h' not_mem) := by
-  simp_to_model using getValueCast_insertList_not_mem
-
-theorem get_insertMany_list_mem [LawfulBEq α]
-    {l : List ((a : α) × (β a))} {k k' : α} {k_eq : k == k'} {v : β k}
-    {distinct : l.Pairwise (fun a b => (a.1 == b.1) = false)}
-    {mem : ⟨k,v⟩ ∈ l}
-    {h'}
-    (h : m.1.WF) :
-    (m.insertMany l).1.get k' h' = cast (by congr; apply LawfulBEq.eq_of_beq k_eq) v := by
-  simp_to_model using getValueCast_insertList_mem
-
-theorem get!_insertMany_list_not_mem [LawfulBEq α]
-    {l : List ((a : α) × (β a))} {k : α} [Inhabited (β k)]
-    {not_mem : (l.map (Sigma.fst)).contains k = false}
-    (h : m.1.WF) :
-    (m.insertMany l).1.get! k = m.get! k := by
-  simp_to_model using getValueCast!_insertList_not_mem
-
-theorem get!_insertMany_list_mem [LawfulBEq α]
-    {l : List ((a : α) × (β a))} {k k' : α} {k_eq : k == k'} {v : β k} [Inhabited (β k')]
-    {distinct : l.Pairwise (fun a b => (a.1 == b.1) = false)}
-    {mem : ⟨k,v⟩ ∈ l}
-    (h : m.1.WF) :
-    (m.insertMany l).1.get! k' = cast (by congr; apply LawfulBEq.eq_of_beq k_eq) v := by
-  simp_to_model using getValueCast!_insertList_mem
-
-theorem getD_insertMany_list_not_mem [LawfulBEq α]
-    {l : List ((a : α) × (β a))} {k : α} {fallback : β k}
-    {not_mem : (l.map (Sigma.fst)).contains k = false}
-    (h : m.1.WF) :
-    (m.insertMany l).1.getD k fallback = m.getD k fallback := by
-  simp_to_model using getValueCastD_insertList_not_mem
-
-theorem getD_insertMany_list_mem [LawfulBEq α]
-    {l : List ((a : α) × (β a))} {k k' : α} {k_eq : k == k'} {v : β k} {fallback : β k'}
-    {distinct : l.Pairwise (fun a b => (a.1 == b.1) = false)}
-    {mem : ⟨k,v⟩ ∈ l}
-    (h : m.1.WF) :
-    (m.insertMany l).1.getD k' fallback = cast (by congr; apply LawfulBEq.eq_of_beq k_eq) v := by
-  simp_to_model using getValueCastD_insertList_mem
-
-theorem getKey?_insertMany_list_not_mem [EquivBEq α] [LawfulHashable α] (h : m.1.WF)
-    {l : List ((a : α) × (β a))} {k : α}
-    {not_mem : (l.map Sigma.fst).contains k = false} :
-    (m.insertMany l).1.getKey? k = m.getKey? k := by
-  simp_to_model using List.getKey?_insertList_not_mem
-
-theorem getKey?_insertMany_list_mem [EquivBEq α] [LawfulHashable α] (h : m.1.WF)
-    {l : List ((a : α) × (β a))}
-    {k k' : α} {k_beq : k == k'}
-    {distinct : l.Pairwise (fun a b => (a.1 == b.1) = false)}
-    {mem : k ∈ (l.map Sigma.fst)} :
-    (m.insertMany l).1.getKey? k' = some k := by
-  simp_to_model using List.getKey?_insertList_mem
-
-theorem getKey_insertMany_list_not_mem [EquivBEq α] [LawfulHashable α] (h : m.1.WF)
-    {l : List ((a : α) × (β a))} {k : α}
-    {not_mem : (l.map Sigma.fst).contains k = false}
+theorem get_insertMany_list_of_contains_eq_false [LawfulBEq α] (h : m.1.WF)
+    {l : List ((a : α) × β a)} {k : α}
+    (contains : (l.map (Sigma.fst)).contains k = false)
     {h'} :
-    (m.insertMany l).1.getKey k h' = m.getKey k (contains_of_contains_insertMany_list _ h h' not_mem) := by
-  simp_to_model using List.getKey_insertList_not_mem
+    (m.insertMany l).1.get k h' =
+    m.get k (contains_of_contains_insertMany_list _ h h' contains) := by
+  simp_to_model using getValueCast_insertList_of_contains_eq_false
 
-theorem getKey_insertMany_list_mem [EquivBEq α] [LawfulHashable α] (h : m.1.WF)
-    {l : List ((a : α) × (β a))}
-    {k k' : α} {k_beq : k == k'}
-    {distinct : l.Pairwise (fun a b => (a.1 == b.1) = false)}
-    {mem : k ∈ (l.map Sigma.fst)}
+theorem get_insertMany_list_of_mem [LawfulBEq α] (h : m.1.WF)
+    {l : List ((a : α) × β a)} {k k' : α} (k_beq : k == k') {v : β k}
+    (distinct : l.Pairwise (fun a b => (a.1 == b.1) = false))
+    (mem : ⟨k, v⟩ ∈ l)
+    {h'} :
+    (m.insertMany l).1.get k' h' = cast (by congr; apply LawfulBEq.eq_of_beq k_beq) v := by
+  simp_to_model using getValueCast_insertList_of_mem
+
+theorem get!_insertMany_list_of_contains_eq_false [LawfulBEq α] (h : m.1.WF)
+    {l : List ((a : α) × β a)} {k : α} [Inhabited (β k)]
+    (h' : (l.map (Sigma.fst)).contains k = false) :
+    (m.insertMany l).1.get! k = m.get! k := by
+  simp_to_model using getValueCast!_insertList_of_contains_eq_false
+
+theorem get!_insertMany_list_of_mem [LawfulBEq α] (h : m.1.WF)
+    {l : List ((a : α) × β a)} {k k' : α} (k_beq : k == k') {v : β k} [Inhabited (β k')]
+    (distinct : l.Pairwise (fun a b => (a.1 == b.1) = false))
+    (mem : ⟨k, v⟩ ∈ l) :
+    (m.insertMany l).1.get! k' = cast (by congr; apply LawfulBEq.eq_of_beq k_beq) v := by
+  simp_to_model using getValueCast!_insertList_of_mem
+
+theorem getD_insertMany_list_of_contains_eq_false [LawfulBEq α] (h : m.1.WF)
+    {l : List ((a : α) × β a)} {k : α} {fallback : β k}
+    (not_mem : (l.map (Sigma.fst)).contains k = false) :
+    (m.insertMany l).1.getD k fallback = m.getD k fallback := by
+  simp_to_model using getValueCastD_insertList_of_contains_eq_false
+
+theorem getD_insertMany_list_of_mem [LawfulBEq α] (h : m.1.WF)
+    {l : List ((a : α) × β a)} {k k' : α} (k_beq : k == k') {v : β k} {fallback : β k'}
+    (distinct : l.Pairwise (fun a b => (a.1 == b.1) = false))
+    (mem : ⟨k, v⟩ ∈ l) :
+    (m.insertMany l).1.getD k' fallback = cast (by congr; apply LawfulBEq.eq_of_beq k_beq) v := by
+  simp_to_model using getValueCastD_insertList_of_mem
+
+theorem getKey?_insertMany_list_of_contains_eq_false [EquivBEq α] [LawfulHashable α] (h : m.1.WF)
+    {l : List ((a : α) × β a)} {k : α}
+    (h : (l.map Sigma.fst).contains k = false) :
+    (m.insertMany l).1.getKey? k = m.getKey? k := by
+  simp_to_model using getKey?_insertList_of_contains_eq_false
+
+theorem getKey?_insertMany_list_of_mem [EquivBEq α] [LawfulHashable α] (h : m.1.WF)
+    {l : List ((a : α) × β a)}
+    {k k' : α} (k_beq : k == k')
+    (distinct : l.Pairwise (fun a b => (a.1 == b.1) = false))
+    (mem : k ∈ (l.map Sigma.fst)) :
+    (m.insertMany l).1.getKey? k' = some k := by
+  simp_to_model using getKey?_insertList_of_mem
+
+theorem getKey_insertMany_list_of_contains_eq_false [EquivBEq α] [LawfulHashable α] (h : m.1.WF)
+    {l : List ((a : α) × β a)} {k : α}
+    (h₁ : (l.map Sigma.fst).contains k = false)
+    {h'} :
+    (m.insertMany l).1.getKey k h' =
+    m.getKey k (contains_of_contains_insertMany_list _ h h' h₁) := by
+  simp_to_model using getKey_insertList_of_contains_eq_false
+
+theorem getKey_insertMany_list_of_mem [EquivBEq α] [LawfulHashable α] (h : m.1.WF)
+    {l : List ((a : α) × β a)}
+    {k k' : α} (k_beq : k == k')
+    (distinct : l.Pairwise (fun a b => (a.1 == b.1) = false))
+    (mem : k ∈ (l.map Sigma.fst))
     {h'} :
     (m.insertMany l).1.getKey k' h' = k := by
-  simp_to_model using List.getKey_insertList_mem
+  simp_to_model using getKey_insertList_of_mem
 
-theorem getKey!_insertMany_list_not_mem [EquivBEq α] [LawfulHashable α] [Inhabited α] (h : m.1.WF)
-    {l : List ((a : α) × (β a))} {k : α}
-    {not_mem : (l.map Sigma.fst).contains k = false} :
+theorem getKey!_insertMany_list_of_contains_eq_false [EquivBEq α] [LawfulHashable α] [Inhabited α]
+    (h : m.1.WF) {l : List ((a : α) × β a)} {k : α}
+    (h' : (l.map Sigma.fst).contains k = false) :
     (m.insertMany l).1.getKey! k = m.getKey! k := by
-  simp_to_model using List.getKey!_insertList_not_mem
+  simp_to_model using getKey!_insertList_of_contains_eq_false
 
-theorem getKey!_insertMany_list_mem [EquivBEq α] [LawfulHashable α] [Inhabited α] (h : m.1.WF)
-    {l : List ((a : α) × (β a))}
-    {k k' : α} {k_beq : k == k'}
-    {distinct : l.Pairwise (fun a b => (a.1 == b.1) = false)}
-    {mem : k ∈ (l.map Sigma.fst)} :
+theorem getKey!_insertMany_listof_mem [EquivBEq α] [LawfulHashable α] [Inhabited α] (h : m.1.WF)
+    {l : List ((a : α) × β a)}
+    {k k' : α} (k_beq : k == k')
+    (distinct : l.Pairwise (fun a b => (a.1 == b.1) = false))
+    (mem : k ∈ (l.map Sigma.fst)) :
     (m.insertMany l).1.getKey! k' = k := by
-  simp_to_model using List.getKey!_insertList_mem
+  simp_to_model using getKey!_insertList_of_mem
 
-theorem getKeyD_insertMany_list_not_mem [EquivBEq α] [LawfulHashable α] (h : m.1.WF)
-    {l : List ((a : α) × (β a))} {k fallback : α}
-    {not_mem : (l.map Sigma.fst).contains k = false} :
+theorem getKeyD_insertMany_list_of_contains_eq_false [EquivBEq α] [LawfulHashable α] (h : m.1.WF)
+    {l : List ((a : α) × β a)} {k fallback : α}
+    (h' : (l.map Sigma.fst).contains k = false) :
     (m.insertMany l).1.getKeyD k fallback = m.getKeyD k fallback := by
-  simp_to_model using List.getKeyD_insertList_not_mem
+  simp_to_model using getKeyD_insertList_of_contains_eq_false
 
-theorem getKeyD_insertMany_list_mem [EquivBEq α] [LawfulHashable α] (h : m.1.WF)
-    {l : List ((a : α) × (β a))}
-    {k k' fallback : α} {k_beq : k == k'}
-    {distinct : l.Pairwise (fun a b => (a.1 == b.1) = false)}
-    {mem : k ∈ (l.map Sigma.fst)} :
+theorem getKeyD_insertMany_list_of_mem [EquivBEq α] [LawfulHashable α] (h : m.1.WF)
+    {l : List ((a : α) × β a)}
+    {k k' fallback : α} (k_beq : k == k')
+    (distinct : l.Pairwise (fun a b => (a.1 == b.1) = false))
+    (mem : k ∈ (l.map Sigma.fst)) :
     (m.insertMany l).1.getKeyD k' fallback = k := by
-  simp_to_model using List.getKeyD_insertList_mem
+  simp_to_model using getKeyD_insertList_of_mem
 
-theorem size_insertMany_list [EquivBEq α] [LawfulHashable α]
-    {l : List ((a : α) × (β a))}
-    {distinct : List.Pairwise (fun a b => (a.1 == b.1) = false) l}
-    (h : m.1.WF) :
-    (∀ (a : α), ¬ (m.contains a = true ∧ (l.map Sigma.fst).contains a = true)) →
+theorem size_insertMany_list [EquivBEq α] [LawfulHashable α] (h : m.1.WF)
+    {l : List ((a : α) × β a)} {distinct : List.Pairwise (fun a b => (a.1 == b.1) = false) l}:
+    (∀ (a : α), ¬ (m.contains a ∧ (l.map Sigma.fst).contains a)) →
     (m.insertMany l).1.1.size = m.1.size + l.length := by
-  simp_to_model using List.insertList_length
+  simp_to_model using length_insertList
 
-theorem insertMany_list_notEmpty_if_map_notEmpty [EquivBEq α] [LawfulHashable α]
-    {l : List ((a : α) × (β a))} (h : m.1.WF) :
+theorem isEmpty_insertMany_list_eq_false_of_isEmpty_eq_false [EquivBEq α] [LawfulHashable α]
+    (h : m.1.WF) {l : List ((a : α) × β a)}:
     (m.1.isEmpty = false) → (m.insertMany l).1.1.isEmpty  = false := by
-  simp_to_model using List.insertList_not_isEmpty_if_start_not_isEmpty
+  simp_to_model using isEmpty_insertList_eq_false_of_isEmpty_eq_false
 
-theorem insertMany_list_isEmpty [EquivBEq α] [LawfulHashable α]
-    {l : List ((a : α) × (β a))} (h : m.1.WF) :
+theorem isEmpty_insertMany_list [EquivBEq α] [LawfulHashable α] (h : m.1.WF)
+    {l : List ((a : α) × β a)} :
     (m.insertMany l).1.1.isEmpty ↔ m.1.isEmpty ∧ l.isEmpty := by
-  simp_to_model using List.insertList_isEmpty
+  simp_to_model using isEmpty_insertList
 
 section
 variable {β: Type v} (m: Raw₀ α (fun _ => β))
 
-theorem get?_insertMany_list_not_mem_const [EquivBEq α] [LawfulHashable α]
-    {l : List ((_ : α) × β)} {k : α}
-    {not_mem : (l.map Sigma.fst).contains k = false}
-    (h : m.1.WF) :
+theorem get?_insertMany_list_of_contains_eq_false_const [EquivBEq α] [LawfulHashable α] (h : m.1.WF)
+    {l : List ((_ : α) × β)} {k : α} (h : (l.map Sigma.fst).contains k = false) :
     Const.get? (m.insertMany l).1 k = Const.get? m k := by
-  simp_to_model using getValue?_insertList_not_mem
+  simp_to_model using getValue?_insertList_of_contains_eq_false
 
-theorem get?_insertMany_list_mem_const [EquivBEq α] [LawfulHashable α]
-    {l : List ((_ : α) × β)} {k k' : α} {k_eq:  k == k'} {v : β} {mem : ⟨k,v⟩ ∈ l}
-    {distinct : List.Pairwise (fun a b => (a.1 == b.1) = false ) l} (h : m.1.WF):
+theorem get?_insertMany_list_of_mem_const [EquivBEq α] [LawfulHashable α] (h : m.1.WF)
+    {l : List ((_ : α) × β)} {k k' : α} (k_beq : k == k') {v : β} (mem : ⟨k, v⟩ ∈ l)
+    (distinct : List.Pairwise (fun a b => (a.1 == b.1) = false ) l) :
     Const.get? (m.insertMany l).1 k' = v := by
-  simp_to_model using getValue?_insertList_mem
+  simp_to_model using getValue?_insertList_of_mem
 
-theorem get_insertMany_list_not_mem_const [EquivBEq α] [LawfulHashable α]
+theorem get_insertMany_list_of_contains_eq_false_const [EquivBEq α] [LawfulHashable α] (h : m.1.WF)
     {l : List ((_ : α) × β)} {k : α}
-    {not_mem : (l.map Sigma.fst).contains k = false}
-    (h : m.1.WF) {h'}:
-    Const.get (m.insertMany l).1 k h' = Const.get m k (contains_of_contains_insertMany_list _ h h' not_mem) := by
-  simp_to_model using getValue_insertList_not_mem
+    (h₁ : (l.map Sigma.fst).contains k = false) {h'}:
+    Const.get (m.insertMany l).1 k h' =
+    Const.get m k (contains_of_contains_insertMany_list _ h h' h₁) := by
+  simp_to_model using getValue_insertList_of_contains_eq_false
 
-theorem get_insertMany_list_mem_const [EquivBEq α] [LawfulHashable α]
-    {l : List ((_ : α) × β)} {k k' : α} {k_eq:  k == k'} {v : β} {mem : ⟨k,v⟩ ∈ l}
-    {distinct : List.Pairwise (fun a b => (a.1 == b.1) = false ) l} (h : m.1.WF) {h'}:
+theorem get_insertMany_list_of_mem_const [EquivBEq α] [LawfulHashable α] (h : m.1.WF)
+    {l : List ((_ : α) × β)} {k k' : α} (k_beq : k == k') {v : β} (mem : ⟨k, v⟩ ∈ l)
+    (distinct : List.Pairwise (fun a b => (a.1 == b.1) = false ) l) {h'}:
     Const.get (m.insertMany l).1 k' h' = v := by
-  simp_to_model using getValue_insertList_mem
+  simp_to_model using getValue_insertList_of_mem
 
-theorem get!_insertMany_list_not_mem_const [EquivBEq α] [LawfulHashable α] [Inhabited β]
-    {l : List ((_ : α) × β)} {k : α}
-    {not_mem : (l.map Sigma.fst).contains k = false}
-    (h : m.1.WF) :
+theorem get!_insertMany_list_of_contains_eq_false_const [EquivBEq α] [LawfulHashable α]
+    [Inhabited β] (h : m.1.WF) {l : List ((_ : α) × β)} {k : α}
+    (h' : (l.map Sigma.fst).contains k = false) :
     Const.get! (m.insertMany l).1 k = Const.get! m k := by
-  simp_to_model using getValue!_insertList_not_mem
+  simp_to_model using getValue!_insertList_of_contains_eq_false
 
-theorem get!_insertMany_list_mem_const [EquivBEq α] [LawfulHashable α] [Inhabited β]
-    {l : List ((_ : α) × β)} {k k' : α} {k_eq:  k == k'} {v : β} {mem : ⟨k,v⟩ ∈ l}
-    {distinct : List.Pairwise (fun a b => (a.1 == b.1) = false ) l} (h : m.1.WF):
+theorem get!_insertMany_list_of_mem_const [EquivBEq α] [LawfulHashable α] [Inhabited β] (h : m.1.WF)
+    {l : List ((_ : α) × β)} {k k' : α} (k_beq : k == k') {v : β} (mem: ⟨k, v⟩ ∈ l)
+    (distinct : List.Pairwise (fun a b => (a.1 == b.1) = false ) l) :
     Const.get! (m.insertMany l).1 k' = v := by
-  simp_to_model using getValue!_insertList_mem
+  simp_to_model using getValue!_insertList_of_mem
 
-theorem getD_insertMany_list_not_mem_const [EquivBEq α] [LawfulHashable α]
+theorem getD_insertMany_list_of_contains_eq_false_const [EquivBEq α] [LawfulHashable α] (h : m.1.WF)
     {l : List ((_ : α) × β)} {k : α} {fallback : β}
-    {not_mem : (l.map Sigma.fst).contains k = false}
-    (h : m.1.WF) :
+    (h' : (l.map Sigma.fst).contains k = false) :
     Const.getD (m.insertMany l).1 k fallback = Const.getD m k fallback:= by
-  simp_to_model using getValueD_insertList_not_mem
+  simp_to_model using getValueD_insertList_of_contains_eq_false
 
-theorem getD_insertMany_list_mem_const [EquivBEq α] [LawfulHashable α]
-    {l : List ((_ : α) × β)} {k k' : α} {k_eq:  k == k'} {v fallback: β} {mem : ⟨k,v⟩ ∈ l}
-    {distinct : List.Pairwise (fun a b => (a.1 == b.1) = false ) l} (h : m.1.WF):
+theorem getD_insertMany_list_of_mem_const [EquivBEq α] [LawfulHashable α] (h : m.1.WF)
+    {l : List ((_ : α) × β)} {k k' : α} (k_beq : k == k') {v fallback: β} (mem: ⟨k, v⟩ ∈ l)
+    (distinct : List.Pairwise (fun a b => (a.1 == b.1) = false ) l) :
     Const.getD (m.insertMany l).1 k' fallback = v := by
-  simp_to_model using getValueD_insertList_mem
+  simp_to_model using getValueD_insertList_of_mem
 
 namespace Const
 @[simp]
-theorem insertMany_list_nil :
+theorem insertMany_nil :
     insertMany m [] = m := by
   simp [insertMany, Id.run]
 
 @[simp]
-theorem insertMany_list_singleton [EquivBEq α] [LawfulHashable α] {k : α} {v : β} :
-    insertMany m [⟨k,v⟩] = m.insert k v := by
+theorem insertMany_list_singleton {k : α} {v : β} :
+    insertMany m [⟨k, v⟩] = m.insert k v := by
   simp [insertMany, Id.run]
 
-theorem insertMany_list_cons {l : List (α × β)} {k : α} {v : β} :
-    (insertMany m (⟨k,v⟩ :: l)).1 = (insertMany (m.insert k v) l).1 := by
+theorem insertMany_cons {l : List (α × β)} {k : α} {v : β} :
+    (insertMany m (⟨k, v⟩ :: l)).1 = (insertMany (m.insert k v) l).1 := by
   simp only [insertMany_eq_insertListₘ]
   cases l with
   | nil => simp [insertListₘ]
   | cons hd tl => simp [insertListₘ]
 
-theorem contains_insertMany_list [EquivBEq α] [LawfulHashable α]  {l : List (α × β)} {k : α} (h : m.1.WF) :
+theorem contains_insertMany_list [EquivBEq α] [LawfulHashable α] (h : m.1.WF)
+    {l : List (α × β)} {k : α} :
     (Const.insertMany m l).1.contains k = (m.contains k || (l.map Prod.fst).contains k) := by
-  simp_to_model using List.containsKey_insertListConst
+  simp_to_model using containsKey_insertListConst
 
-theorem contains_of_contains_insertMany_list [EquivBEq α] [LawfulHashable α] (h : m.1.WF) {l : List ( α × β )} {k : α} :
+theorem contains_of_contains_insertMany_list [EquivBEq α] [LawfulHashable α] (h : m.1.WF)
+    {l : List ( α × β )} {k : α} :
     (insertMany m l).1.contains k → (l.map Prod.fst).contains k = false → m.contains k := by
-  simp_to_model using List.containsKey_of_containsKey_insertListConst
+  simp_to_model using containsKey_of_containsKey_insertListConst
 
-theorem getKey?_insertMany_list_not_mem [EquivBEq α] [LawfulHashable α] (h : m.1.WF)
+theorem getKey?_insertMany_list_of_contains_eq_false [EquivBEq α] [LawfulHashable α] (h : m.1.WF)
     {l : List (α × β)} {k : α}
-    {not_mem : (l.map Prod.fst).contains k = false} :
+    (h' : (l.map Prod.fst).contains k = false) :
     (insertMany m l).1.getKey? k = m.getKey? k := by
-  simp_to_model using List.getKey?_insertListConst_not_mem
+  simp_to_model using getKey?_insertListConst_of_contains_eq_false
 
-theorem getKey?_insertMany_list_mem [EquivBEq α] [LawfulHashable α] (h : m.1.WF)
+theorem getKey?_insertMany_list_of_mem [EquivBEq α] [LawfulHashable α] (h : m.1.WF)
     {l : List  (α × β)}
-    {k k' : α} {k_beq : k == k'}
-    {distinct : l.Pairwise (fun a b => (a.1 == b.1) = false)}
-    {mem : k ∈ (l.map Prod.fst)} :
+    {k k' : α} (k_beq : k == k')
+    (distinct : l.Pairwise (fun a b => (a.1 == b.1) = false))
+    (mem : k ∈ (l.map Prod.fst)) :
     (insertMany m l).1.getKey? k' = some k := by
-  simp_to_model using List.getKey?_insertListConst_mem
+  simp_to_model using getKey?_insertListConst_of_mem
 
-theorem getKey_insertMany_list_not_mem [EquivBEq α] [LawfulHashable α] (h : m.1.WF)
+theorem getKey_insertMany_list_of_contains_eq_false [EquivBEq α] [LawfulHashable α] (h : m.1.WF)
     {l : List (α × β)} {k : α}
-    {not_mem : (l.map Prod.fst).contains k = false}
+    {h₁ : (l.map Prod.fst).contains k = false}
     {h'} :
-    (insertMany m l).1.getKey k h' = m.getKey k (contains_of_contains_insertMany_list _ h h' not_mem) := by
-  simp_to_model using List.getKey_insertListConst_not_mem
+    (insertMany m l).1.getKey k h' =
+    m.getKey k (contains_of_contains_insertMany_list _ h h' h₁) := by
+  simp_to_model using getKey_insertListConst_of_contains_eq_false
 
-theorem getKey_insertMany_list_mem [EquivBEq α] [LawfulHashable α] (h : m.1.WF)
+theorem getKey_insertMany_list_of_mem [EquivBEq α] [LawfulHashable α] (h : m.1.WF)
     {l : List (α × β)}
-    {k k' : α} {k_beq : k == k'}
-    {distinct : l.Pairwise (fun a b => (a.1 == b.1) = false)}
-    {mem : k ∈ (l.map Prod.fst)}
+    {k k' : α} (k_beq : k == k')
+    (distinct : l.Pairwise (fun a b => (a.1 == b.1) = false))
+    (mem : k ∈ (l.map Prod.fst))
     {h'} :
     (insertMany m l).1.getKey k' h' = k := by
-  simp_to_model using List.getKey_insertListConst_mem
+  simp_to_model using getKey_insertListConst_of_mem
 
-theorem getKey!_insertMany_list_not_mem [EquivBEq α] [LawfulHashable α] [Inhabited α] (h : m.1.WF)
-    {l : List (α × β)} {k : α}
-    {not_mem : (l.map Prod.fst).contains k = false} :
+theorem getKey!_insertMany_list_of_contains_eq_false [EquivBEq α] [LawfulHashable α] [Inhabited α]
+    (h : m.1.WF) {l : List (α × β)} {k : α}
+    (h' : (l.map Prod.fst).contains k = false) :
     (insertMany m l).1.getKey! k = m.getKey! k := by
-  simp_to_model using List.getKey!_insertListConst_not_mem
+  simp_to_model using getKey!_insertListConst_of_contains_eq_false
 
-theorem getKey!_insertMany_list_mem [EquivBEq α] [LawfulHashable α] [Inhabited α] (h : m.1.WF)
+theorem getKey!_insertMany_list_of_mem [EquivBEq α] [LawfulHashable α] [Inhabited α] (h : m.1.WF)
     {l : List (α × β)}
-    {k k' : α} {k_beq : k == k'}
-    {distinct : l.Pairwise (fun a b => (a.1 == b.1) = false)}
-    {mem : k ∈ (l.map Prod.fst)} :
+    {k k' : α} (k_beq : k == k')
+    (distinct : l.Pairwise (fun a b => (a.1 == b.1) = false))
+    (mem : k ∈ (l.map Prod.fst)) :
     (insertMany m l).1.getKey! k' = k := by
-  simp_to_model using List.getKey!_insertListConst_mem
+  simp_to_model using getKey!_insertListConst_of_mem
 
-theorem getKeyD_insertMany_list_not_mem [EquivBEq α] [LawfulHashable α] (h : m.1.WF)
+theorem getKeyD_insertMany_list_of_contains_eq_false [EquivBEq α] [LawfulHashable α] (h : m.1.WF)
     {l : List (α × β)} {k fallback : α}
-    {not_mem : (l.map Prod.fst).contains k = false} :
+    (h' : (l.map Prod.fst).contains k = false) :
     (insertMany m l).1.getKeyD k fallback = m.getKeyD k fallback := by
-  simp_to_model using List.getKeyD_insertListConst_not_mem
+  simp_to_model using getKeyD_insertListConst_of_contains_eq_false
 
-theorem getKeyD_insertMany_list_mem [EquivBEq α] [LawfulHashable α] (h : m.1.WF)
+theorem getKeyD_insertMany_list_of_mem [EquivBEq α] [LawfulHashable α] (h : m.1.WF)
     {l : List (α × β)}
-    {k k' fallback : α} {k_beq : k == k'}
-    {distinct : l.Pairwise (fun a b => (a.1 == b.1) = false)}
-    {mem : k ∈ (l.map Prod.fst)} :
+    {k k' fallback : α} (k_beq : k == k')
+    (distinct : l.Pairwise (fun a b => (a.1 == b.1) = false))
+    (mem : k ∈ (l.map Prod.fst)) :
     (insertMany m l).1.getKeyD k' fallback = k := by
-  simp_to_model using List.getKeyD_insertListConst_mem
+  simp_to_model using getKeyD_insertListConst_of_mem
 
-theorem size_insertMany_list [EquivBEq α] [LawfulHashable α]
+theorem size_insertMany_list [EquivBEq α] [LawfulHashable α] (h : m.1.WF)
     {l : List (α × β)}
-    {distinct : List.Pairwise (fun a b => (a.1 == b.1) = false) l}
-    (h : m.1.WF) :
-    (∀ (a : α), ¬ (m.contains a = true ∧ (l.map Prod.fst).contains a = true)) →
+    {distinct : List.Pairwise (fun a b => (a.1 == b.1) = false) l} :
+    (∀ (a : α), ¬ (m.contains a ∧ (l.map Prod.fst).contains a)) →
     (insertMany m l).1.1.size = m.1.size + l.length := by
-  simp_to_model using List.insertListConst_length
+  simp_to_model using length_insertListConst
 
-theorem insertMany_list_notEmpty_if_map_notEmpty [EquivBEq α] [LawfulHashable α]
-    {l : List (α × β)} (h : m.1.WF) :
+theorem isEmpty_insertMany_list_eq_false_of_isEmpty_eq_false [EquivBEq α] [LawfulHashable α]
+    (h : m.1.WF) {l : List (α × β)} :
     (m.1.isEmpty = false) → (insertMany m l).1.1.isEmpty  = false := by
-  simp_to_model using List.insertListConst_not_isEmpty_if_start_not_isEmpty
+  simp_to_model using isEmpty_insertListConst_eq_false_of_isEmpty_eq_false
 
-theorem insertMany_list_isEmpty [EquivBEq α] [LawfulHashable α]
-    {l : List (α × β)} (h : m.1.WF) :
+theorem isEmpty_insertMany_list [EquivBEq α] [LawfulHashable α] (h : m.1.WF)
+    {l : List (α × β)} :
     (insertMany m l).1.1.isEmpty ↔ m.1.isEmpty ∧ l.isEmpty := by
-  simp_to_model using List.insertListConst_isEmpty
+  simp_to_model using isEmpty_insertListConst
 
-theorem get?_insertMany_list_not_mem_const [EquivBEq α] [LawfulHashable α]
+theorem get?_insertMany_list_of_contains_eq_false [EquivBEq α] [LawfulHashable α] (h : m.1.WF)
     {l : List (α × β)} {k : α}
-    {not_mem : (l.map Prod.fst).contains k = false}
-    (h : m.1.WF) :
+    (h' : (l.map Prod.fst).contains k = false) :
     get? (insertMany m l).1 k = get? m k := by
-  simp_to_model using getValue?_insertListConst_not_mem
+  simp_to_model using getValue?_insertListConst_of_contains_eq_false
 
-theorem get?_insertMany_list_mem_const [EquivBEq α] [LawfulHashable α]
-    {l : List (α × β)} {k k' : α} {k_eq:  k == k'} {v : β} {mem : ⟨k,v⟩ ∈ l}
-    {distinct : List.Pairwise (fun a b => (a.1 == b.1) = false ) l} (h : m.1.WF):
+theorem get?_insertMany_list_of_mem_const [EquivBEq α] [LawfulHashable α] (h : m.1.WF)
+    {l : List (α × β)} {k k' : α} (k_beq : k == k') {v : β} (mem: ⟨k, v⟩ ∈ l)
+    (distinct : List.Pairwise (fun a b => (a.1 == b.1) = false ) l) :
     get? (insertMany m l).1 k' = v := by
-  simp_to_model using getValue?_insertListConst_mem
+  simp_to_model using getValue?_insertListConst_of_mem
 
-theorem get_insertMany_list_not_mem_const [EquivBEq α] [LawfulHashable α]
+theorem get_insertMany_list_of_contains_eq_false [EquivBEq α] [LawfulHashable α] (h : m.1.WF)
     {l : List (α × β)} {k : α}
-    {not_mem : (l.map Prod.fst).contains k = false}
-    (h : m.1.WF) {h'}:
-    get (insertMany m l).1 k h' = get m k (contains_of_contains_insertMany_list _ h h' not_mem) := by
-  simp_to_model using getValue_insertListConst_not_mem
+    (h₁ : (l.map Prod.fst).contains k = false)
+    {h'}:
+    get (insertMany m l).1 k h' = get m k (contains_of_contains_insertMany_list _ h h' h₁) := by
+  simp_to_model using getValue_insertListConst_of_contains_eq_false
 
-theorem get_insertMany_list_mem_const [EquivBEq α] [LawfulHashable α]
-    {l : List (α × β)} {k k' : α} {k_eq:  k == k'} {v : β} {mem : ⟨k,v⟩ ∈ l}
-    {distinct : List.Pairwise (fun a b => (a.1 == b.1) = false ) l} (h : m.1.WF) {h'}:
+theorem get_insertMany_list_of_mem_const [EquivBEq α] [LawfulHashable α] (h : m.1.WF)
+    {l : List (α × β)} {k k' : α} (k_beq : k == k') {v : β} (mem: ⟨k, v⟩ ∈ l)
+    (distinct : List.Pairwise (fun a b => (a.1 == b.1) = false ) l) {h'}:
     get (insertMany m l).1 k' h' = v := by
-  simp_to_model using getValue_insertListConst_mem
+  simp_to_model using getValue_insertListConst_of_mem
 
-theorem get!_insertMany_list_not_mem_const [EquivBEq α] [LawfulHashable α] [Inhabited β]
-    {l : List (α × β)} {k : α}
-    {not_mem : (l.map Prod.fst).contains k = false}
-    (h : m.1.WF) :
+theorem get!_insertMany_list_of_contains_eq_false_const [EquivBEq α] [LawfulHashable α]
+    [Inhabited β]  (h : m.1.WF) {l : List (α × β)} {k : α}
+    (h' : (l.map Prod.fst).contains k = false) :
     get! (insertMany m l).1 k = get! m k := by
-  simp_to_model using getValue!_insertListConst_not_mem
+  simp_to_model using getValue!_insertListConst_of_contains_eq_false
 
-theorem get!_insertMany_list_mem_const [EquivBEq α] [LawfulHashable α] [Inhabited β]
-    {l : List (α × β)} {k k' : α} {k_eq:  k == k'} {v : β} {mem : ⟨k,v⟩ ∈ l}
-    {distinct : List.Pairwise (fun a b => (a.1 == b.1) = false ) l} (h : m.1.WF):
+theorem get!_insertMany_list_of_mem_const [EquivBEq α] [LawfulHashable α] [Inhabited β] (h : m.1.WF)
+    {l : List (α × β)} {k k' : α} (k_beq : k == k') {v : β} (mem: ⟨k, v⟩ ∈ l)
+    (distinct : List.Pairwise (fun a b => (a.1 == b.1) = false ) l) :
     get! (insertMany m l).1 k' = v := by
-  simp_to_model using getValue!_insertListConst_mem
+  simp_to_model using getValue!_insertListConst_of_mem
 
-theorem getD_insertMany_list_not_mem_const [EquivBEq α] [LawfulHashable α]
+theorem getD_insertMany_list_of_contains_eq_false_const [EquivBEq α] [LawfulHashable α] (h : m.1.WF)
     {l : List (α × β)} {k : α} {fallback : β}
-    {not_mem : (l.map Prod.fst).contains k = false}
-    (h : m.1.WF) :
+    (h' : (l.map Prod.fst).contains k = false) :
     getD (insertMany m l).1 k fallback = getD m k fallback:= by
-  simp_to_model using getValueD_insertListConst_not_mem
+  simp_to_model using getValueD_insertListConst_of_contains_eq_false
 
-theorem getD_insertMany_list_mem_const [EquivBEq α] [LawfulHashable α]
-    {l : List (α × β)} {k k' : α} {k_eq:  k == k'} {v fallback: β} {mem : ⟨k,v⟩ ∈ l}
-    {distinct : List.Pairwise (fun a b => (a.1 == b.1) = false ) l} (h : m.1.WF):
+theorem getD_insertMany_list_of_mem_const [EquivBEq α] [LawfulHashable α] (h : m.1.WF)
+    {l : List (α × β)} {k k' : α} (k_beq : k == k') {v fallback: β} (mem: ⟨k, v⟩ ∈ l)
+    (distinct : List.Pairwise (fun a b => (a.1 == b.1) = false ) l) :
     getD (insertMany m l).1 k' fallback = v := by
-  simp_to_model using getValueD_insertListConst_mem
+  simp_to_model using getValueD_insertListConst_of_mem
 
 variable (m: Raw₀ α (fun _ => Unit))
 
 @[simp]
-theorem insertManyIfNewUnit_list_nil :
+theorem insertManyIfNewUnit_nil :
     insertManyIfNewUnit m [] = m := by
   simp [insertManyIfNewUnit, Id.run]
 
@@ -1224,119 +1215,124 @@ theorem insertManyIfNewUnit_list_singleton [EquivBEq α] [LawfulHashable α] {k 
     insertManyIfNewUnit m [k] = m.insertIfNew k () := by
   simp [insertManyIfNewUnit, Id.run]
 
-theorem contains_insertManyIfNewUnit_list [EquivBEq α] [LawfulHashable α] {l : List α} {k : α} (h : m.1.WF):
+theorem insertManyIfNewUnit_cons {l : List α} {k : α} :
+    (insertManyIfNewUnit m (k :: l)).1 = (insertManyIfNewUnit (m.insertIfNew k ()) l).1 := by
+  simp only [insertManyIfNewUnit_eq_insertListIfNewUnitₘ]
+  cases l with
+  | nil => simp [insertListIfNewUnitₘ]
+  | cons hd tl => simp [insertListIfNewUnitₘ]
+
+theorem contains_insertManyIfNewUnit_list [EquivBEq α] [LawfulHashable α] (h : m.1.WF)
+    {l : List α} {k : α}:
     (insertManyIfNewUnit m l).1.contains k = (m.contains k || l.contains k) := by
   simp_to_model using containsKey_insertListIfNewUnit
 
-theorem contains_of_contains_insertManyIfNewUnit_list [EquivBEq α] [LawfulHashable α] {l : List α} {k : α} (h : m.1.WF)
-    (h₂ : l.contains k = false) : (insertManyIfNewUnit m l).1.contains k = true →  m.contains k := by
+theorem contains_of_contains_insertManyIfNewUnit_list [EquivBEq α] [LawfulHashable α] (h : m.1.WF)
+    {l : List α} {k : α} (h₂ : l.contains k = false) :
+    (insertManyIfNewUnit m l).1.contains k →  m.contains k := by
   simp_to_model using containsKey_of_containsKey_insertListIfNewUnit
 
-theorem getKey?_insertManyIfNewUnit_list_not_mem [EquivBEq α] [LawfulHashable α]
-    {l : List α} {k : α}
-    {not_mem : l.contains k = false} (h : m.1.WF) :
+theorem getKey?_insertManyIfNewUnit_list_of_contains_eq_false [EquivBEq α] [LawfulHashable α]
+    (h : m.1.WF) {l : List α} {k : α} (h' : l.contains k = false) :
     getKey? (insertManyIfNewUnit m l).1 k = getKey? m k := by
-  simp_to_model using getKey?_insertListIfNewUnit_not_mem
+  simp_to_model using getKey?_insertListIfNewUnit_of_contains_eq_false
 
-theorem getKey?_insertManyIfNewUnit_list_mem [EquivBEq α] [LawfulHashable α]
-    {l : List α} {k k' : α} {k_beq : k == k'}
-    {distinct : l.Pairwise (fun a b => (a == b) = false)}
-    {mem : k ∈ l} (h : m.1.WF) : m.contains k = false →
-    getKey? (insertManyIfNewUnit m l).1 k' = some k := by
-  simp_to_model using getKey?_insertListIfNewUnit_mem
+theorem getKey?_insertManyIfNewUnit_list_of_mem_of_contains_eq_false [EquivBEq α] [LawfulHashable α]
+    (h : m.1.WF) {l : List α} {k k' : α} (k_beq : k == k')
+    (distinct : l.Pairwise (fun a b => (a == b) = false)) (mem : k ∈ l) :
+    m.contains k = false → getKey? (insertManyIfNewUnit m l).1 k' = some k := by
+  simp_to_model using getKey?_insertListIfNewUnit_of_mem_of_contains_eq_false
 
-theorem getKey?_insertManyIfNewUnit_list_mem_both [EquivBEq α] [LawfulHashable α]
-    {l : List α} {k : α}
-    {distinct : l.Pairwise (fun a b => (a == b) = false)}
-    {mem : l.contains k} (h : m.1.WF):
-    m.contains k = true → getKey? (insertManyIfNewUnit m l).1 k = getKey? m k := by
-  simp_to_model using getKey?_insertListIfNewUnit_mem_both
+theorem getKey?_insertManyIfNewUnit_list_of_mem_of_contains [EquivBEq α] [LawfulHashable α]
+    (h : m.1.WF) {l : List α} {k : α}
+    (distinct : l.Pairwise (fun a b => (a == b) = false))
+    (h': l.contains k) :
+    m.contains k  → getKey? (insertManyIfNewUnit m l).1 k = getKey? m k := by
+  simp_to_model using getKey?_insertListIfNewUnit_of_mem_of_contains
 
-theorem getKey_insertManyIfNewUnit_list_not_mem [EquivBEq α] [LawfulHashable α]
-    {l : List α} {k : α}
-    {not_mem : l.contains k = false}
-    {h'} (h: m.1.WF):
+theorem getKey_insertManyIfNewUnit_list_of_contains_eq_false [EquivBEq α] [LawfulHashable α]
+    (h : m.1.WF) {l : List α} {k : α} (h₁ : l.contains k = false) {h'} :
     getKey (insertManyIfNewUnit m l).1 k h' =
-      getKey m k (contains_of_contains_insertManyIfNewUnit_list m h not_mem h') := by
-  simp_to_model using getKey_insertListIfNewUnit_not_mem
+      getKey m k (contains_of_contains_insertManyIfNewUnit_list m h h₁ h') := by
+  simp_to_model using getKey_insertListIfNewUnit_of_contains_eq_false
 
-theorem getKey_insertManyIfNewUnit_list_mem [EquivBEq α] [LawfulHashable α]
-    {l : List α}
-    {k k' : α} {k_beq : k == k'}
-    {distinct : l.Pairwise (fun a b => (a == b) = false)}
-    {mem : k ∈ l}{h'} (h: m.1.WF):
+theorem getKey_insertManyIfNewUnit_list_of_mem_of_contains_eq_false [EquivBEq α] [LawfulHashable α]
+    (h : m.1.WF) {l : List α}
+    {k k' : α} (k_beq : k == k')
+    (distinct : l.Pairwise (fun a b => (a == b) = false))
+    (mem : k ∈ l) {h'} :
     m.contains k  = false →
     getKey (insertManyIfNewUnit m l).1 k' h' = k := by
-  simp_to_model using getKey_insertListIfNewUnit_mem
+  simp_to_model using getKey_insertListIfNewUnit_of_mem_of_contains_eq_false
 
-theorem getKey_insertManyIfNewUnit_list_mem_both [EquivBEq α] [LawfulHashable α]
-    {l : List α} {k : α}
-    {distinct : l.Pairwise (fun a b => (a == b) = false)}
-    {mem : l.contains k} {mem' : m.contains k = true} {h'} (h : m.1.WF):
+theorem getKey_insertManyIfNewUnit_list_mem_of_mem_of_contains [EquivBEq α] [LawfulHashable α]
+    (h : m.1.WF) {l : List α} {k : α}
+    (distinct : l.Pairwise (fun a b => (a == b) = false))
+    (h': l.contains k) {mem' : m.contains k} {h'} :
     getKey (insertManyIfNewUnit m l).1 k h' = getKey m k mem' := by
-  simp_to_model using getKey_insertListIfNewUnit_mem_both
+  simp_to_model using getKey_insertListIfNewUnit_of_mem_of_contains
 
-theorem getKey!_insertManyIfNewUnit_list_not_mem [EquivBEq α] [LawfulHashable α] [Inhabited α]
-    {l : List α} {k : α}
-    {not_mem : l.contains k = false} (h : m.1.WF) :
+theorem getKey!_insertManyIfNewUnit_list_of_contains_eq_false [EquivBEq α] [LawfulHashable α]
+    [Inhabited α] (h : m.1.WF) {l : List α} {k : α}
+    (h' : l.contains k = false) :
     getKey! (insertManyIfNewUnit m l).1 k = getKey! m k := by
-  simp_to_model using getKey!_insertListIfNewUnit_not_mem
+  simp_to_model using getKey!_insertListIfNewUnit_of_contains_eq_false
 
-theorem getKey!_insertManyIfNewUnit_list_mem [EquivBEq α] [LawfulHashable α] [Inhabited α]
-    {l : List α} {k k' : α} {k_beq : k == k'}
-    {distinct : l.Pairwise (fun a b => (a == b) = false)}
-    {mem : k ∈ l} (h : m.1.WF) : contains m k = false →
+theorem getKey!_insertManyIfNewUnit_list_of_mem_of_contains_eq_false [EquivBEq α] [LawfulHashable α]
+    [Inhabited α] (h : m.1.WF) {l : List α} {k k' : α} (k_beq : k == k')
+    (distinct : l.Pairwise (fun a b => (a == b) = false))
+    (mem : k ∈ l) : contains m k = false →
     getKey! (insertManyIfNewUnit m l).1 k' = k := by
-  simp_to_model using getKey!_insertListIfNewUnit_mem
+  simp_to_model using getKey!_insertListIfNewUnit_of_mem_of_contains_eq_false
 
-theorem getKey!_insertManyIfNewUnit_list_mem_both [EquivBEq α] [LawfulHashable α] [Inhabited α]
-    {l : List α} {k : α}
-    {distinct : l.Pairwise (fun a b => (a == b) = false)}
-    {mem : l.contains k} (h : m.1.WF) : m.contains k = true →
+theorem getKey!_insertManyIfNewUnit_list_mem_of_mem_of_contains [EquivBEq α] [LawfulHashable α]
+    [Inhabited α] (h : m.1.WF) {l : List α} {k : α}
+    (distinct : l.Pairwise (fun a b => (a == b) = false))
+    (h': l.contains k) : m.contains k →
     getKey! (insertManyIfNewUnit m l).1 k = getKey! m k  := by
-  simp_to_model using getKey!_insertListIfNewUnit_mem_both
+  simp_to_model using getKey!_insertListIfNewUnit_of_mem_of_contains
 
-theorem getKeyD_insertManyIfNewUnit_list_not_mem [EquivBEq α] [LawfulHashable α]
-    {l : List α} {k fallback : α}
-    {not_mem : l.contains k = false} (h : m.1.WF):
+theorem getKeyD_insertManyIfNewUnit_list_of_contains_eq_false [EquivBEq α] [LawfulHashable α]
+    (h : m.1.WF) {l : List α} {k fallback : α}
+    (h' : l.contains k = false):
     getKeyD (insertManyIfNewUnit m l).1 k fallback = getKeyD m k fallback := by
-  simp_to_model using getKeyD_insertListIfNewUnit_not_mem
+  simp_to_model using getKeyD_insertListIfNewUnit_of_contains_eq_false
 
-theorem getKeyD_insertManyIfNewUnit_list_mem [EquivBEq α] [LawfulHashable α]
-    {l : List α} {k k' fallback : α} {k_beq : k == k'}
-    {distinct : l.Pairwise (fun a b => (a == b) = false)}
-    {mem : k ∈ l } (h : m.1.WF) : m.contains k = false →
+theorem getKeyD_insertManyIfNewUnit_list_of_mem_of_contains_eq_false [EquivBEq α] [LawfulHashable α]
+    (h : m.1.WF) {l : List α} {k k' fallback : α} (k_beq : k == k')
+    (distinct : l.Pairwise (fun a b => (a == b) = false))
+    {mem : k ∈ l } : m.contains k = false →
     getKeyD (insertManyIfNewUnit m l).1 k' fallback = k := by
-  simp_to_model using getKeyD_insertListIfNewUnit_mem
+  simp_to_model using getKeyD_insertListIfNewUnit_of_mem_of_contains_eq_false
 
-theorem getKeyD_insertManyIfNewUnit_list_mem_both [EquivBEq α] [LawfulHashable α]
-    {l : List α} {k fallback : α}
-    {distinct : l.Pairwise (fun a b => (a == b) = false)}
-    {mem : l.contains k} (h : m.1.WF) : m.contains k = true →
+theorem getKeyD_insertManyIfNewUnit_list_of_mem_of_contains [EquivBEq α] [LawfulHashable α]
+    (h : m.1.WF) {l : List α} {k fallback : α}
+    (distinct : l.Pairwise (fun a b => (a == b) = false))
+    (h': l.contains k) : m.contains k →
     getKeyD (insertManyIfNewUnit m l).1 k fallback = getKeyD m k fallback := by
-  simp_to_model using getKeyD_insertListIfNewUnit_mem_both
+  simp_to_model using getKeyD_insertListIfNewUnit_of_mem_of_contains
 
-theorem insertManyIfNewUnit_list_length [EquivBEq α] [LawfulHashable α]
+theorem size_insertManyIfNewUnit_list [EquivBEq α] [LawfulHashable α] (h : m.1.WF)
     {l : List α}
-    (distinct : List.Pairwise (fun a b => (a == b) = false) l)
-    (h : m.1.WF) : (∀ (a : α), ¬ (m.contains a = true ∧ l.contains a = true)) →
+    (distinct : List.Pairwise (fun a b => (a == b) = false) l):
+    (∀ (a : α), ¬ (m.contains a ∧ l.contains a)) →
     (insertManyIfNewUnit m l).1.1.size = m.1.size + l.length := by
-  simp_to_model using insertListIfNewUnit_length
+  simp_to_model using length_insertListIfNewUnit
 
-theorem insertManyIfNewUnit_list_not_isEmpty_if_start_not_isEmpty [EquivBEq α] [LawfulHashable α]
-    {l : List α} (h : m.1.WF) : m.1.isEmpty = false →
+theorem isEmpty_insertManyIfNewUnit_list_eq_false_of_isEmpty_eq_false [EquivBEq α] [LawfulHashable α]
+    (h : m.1.WF) {l : List α} : m.1.isEmpty = false →
     (insertManyIfNewUnit m l).1.1.isEmpty = false := by
-  simp_to_model using insertListIfNewUnit_not_isEmpty_if_start_not_isEmpty
+  simp_to_model using isEmpty_insertListIfNewUnit_eq_false_of_isEmpty_eq_false
 
-theorem insertManyIfNewUnit_list_isEmpty [EquivBEq α] [LawfulHashable α]
-    {l : List α} (h : m.1.WF) :
+theorem isEmpty_insertManyIfNewUnit_list [EquivBEq α] [LawfulHashable α] (h : m.1.WF)
+    {l : List α} :
     (insertManyIfNewUnit m l).1.1.isEmpty ↔ m.1.isEmpty ∧ l.isEmpty := by
-  simp_to_model using insertListIfNewUnit_isEmpty
+  simp_to_model using isEmpty_insertListIfNewUnit
 
-theorem get?_insertManyIfNewUnit_list [EquivBEq α] [LawfulHashable α]
-    {l : List α} {k : α} (h : m.1.WF) :
+theorem get?_insertManyIfNewUnit_list [EquivBEq α] [LawfulHashable α] (h : m.1.WF)
+    {l : List α} {k : α} :
     get? (insertManyIfNewUnit m l).1 k =
-    if ( m.contains k || l.contains k) then some () else none := by
+    if m.contains k ∨ l.contains k then some () else none := by
   simp_to_model using getValue?_insertListIfNewUnit
 
 theorem getValue_insertManyIfNewUnit_list
